Use Words library to implement Types_s, use pow2_* and other Words library definitions in all files

src/arch/Types_i.fsti
@@ -3,14 +3,17 @@ module Types_i
 open Types_s
 open Collections.Seqs_s
 open Collections.Seqs_i
+open Words_s
+open Words.Four_s
+open Words.Seq_s
 open FStar.Seq
 
 unfold let ( *^ ) = nat32_xor
 unfold let ( *^^ ) = quad32_xor
 
 let quad32_shl32 (q:quad32) : quad32 =
-  let Quad32 v0 v1 v2 v3 = q in
-  Quad32 0 v0 v1 v2
+  let Mkfour v0 v1 v2 v3 = q in
+  Mkfour 0 v0 v1 v2
 
 val lemma_BitwiseXorCommutative (x y:nat32) : Lemma (x *^ y == y *^ x)
 val lemma_BitwiseXorWithZero (n:nat32) : Lemma (n *^ 0 == n)
@@ -27,15 +30,10 @@ val xor_lemmas (_:unit) : Lemma
     (forall (x y z:nat32).{:pattern (x *^ (y *^ z))} x *^ (y *^ z) == (x *^ y) *^ z)
   )
 
-val lemma_quad32_xor (_:unit) : Lemma (forall q . {:pattern quad32_xor q q} quad32_xor q q == Quad32 0 0 0 0)
+val lemma_quad32_xor (_:unit) : Lemma (forall q . {:pattern quad32_xor q q} quad32_xor q q == Mkfour 0 0 0 0)
 
-let quad32_double_lo (q:quad32) : double32 =
-  let Quad32 q0 q1 q2 q3 = q in
-  Double32 q0 q1
-
-let quad32_double_hi (q:quad32) : double32 =
-  let Quad32 q0 q1 q2 q3 = q in
-  Double32 q2 q3
+let quad32_double_lo (q:quad32) : double32 = (four_to_two_two q).lo
+let quad32_double_hi (q:quad32) : double32 = (four_to_two_two q).hi
 
 val lemma_reverse_reverse_bytes_nat32 (n:nat32) :
   Lemma (reverse_bytes_nat32 (reverse_bytes_nat32 n) == n)
@@ -48,13 +46,6 @@ let lemma_reverse_bytes_quad32 (q:quad32) :
 
 val lemma_reverse_reverse_bytes_nat32_seq (s:seq nat32) :
   Lemma (ensures reverse_bytes_nat32_seq (reverse_bytes_nat32_seq s) == s)
-  (decreases %[length s])
   [SMTPat (reverse_bytes_nat32_seq (reverse_bytes_nat32_seq s))]
-  
-val quad32_to_seq (q:quad32) : 
-  Tot (s:seq nat32 { length s == 4 /\ 
-                     (let q' = Quad32 (index s 0) (index s 1) (index s 2) (index s 3) in
-                      q == q')           
-                   })
 
-
+unfold let quad32_to_seq (q:quad32) = four_to_seq_LE q
