src/arch/Types_s.fst
@@ -1,26 +1,14 @@
 module Types_s
 
+open Words_s
+open Words.Four_s
+open Words.Seq_s
 open Collections.Seqs_s
 
-unfold let nat8_max = 0x100
-unfold let nat16_max = 0x10000
-unfold let nat32_max = 0x100000000
-unfold let nat64_max = 0x10000000000000000
-unfold let nat128_max = 0x100000000000000000000000000000000
-
-// Sanity check our constants
-let _ = assert_norm (pow2 8 = nat8_max)
-let _ = assert_norm (pow2 16 = nat16_max)
-let _ = assert_norm (pow2 32 = nat32_max)
-let _ = assert_norm (pow2 64 = nat64_max)
-let _ = assert_norm (pow2 128 = nat128_max)
-
-let natN (n:nat) = x:nat{x < n}
-let nat8 = natN nat8_max
-let nat16 = natN nat16_max
-let nat32 = natN nat32_max
-let nat64 = natN nat64_max
-let nat128 = natN nat128_max
+unfold let nat8 = Words_s.nat8
+unfold let nat16 = Words_s.nat16
+unfold let nat32 = Words_s.nat32
+unfold let nat64 = Words_s.nat64
 
 let add_wrap (#n:nat) (x:natN n) (y:natN n) : natN n = if x + y < n then x + y else x + y - n
 
@@ -35,61 +23,28 @@ assume val ishr : #n:nat -> a:natN n -> s:int -> natN n
 // Alias
 unfold let nat32_xor (x y:nat32) : nat32 = ixor x y
 
-type twobits = i:int{0 <= i && i < 4}
-type bits_of_byte = | Bits_of_Byte :
-  lo:twobits ->
-  mid_lo:twobits ->  
-  mid_hi:twobits ->
-  hi:twobits ->
-  bits_of_byte
+type twobits = natN 4
+type bits_of_byte = four twobits
 
-let byte_to_twobits (b:nat8) =
-  Bits_of_Byte
-    (b % 4)
-    ((b / 4) % 4)
-    ((b / 16) % 4)
-    ((b / 64) % 4)
+unfold let byte_to_twobits (b:nat8) : bits_of_byte = nat_to_four_unfold 2 b
 
-type double32 = | Double32: lo:nat32 -> hi:nat32 -> double32
+type double32 = two nat32
+type quad32 = four nat32
 
-type quad32 = | Quad32:
-  lo:nat32 ->
-  mid_lo:nat32 ->
-  mid_hi:nat32 ->
-  hi:nat32 ->
-  quad32
+let quad32_xor (x y:quad32) : quad32 = four_map2 nat32_xor x y
 
-unfold
-let quad32_map (f:nat32 -> nat32) (x:quad32) : quad32 =
-  let Quad32 x0 x1 x2 x3 = x in
-  Quad32 (f x0) (f x1) (f x2) (f x3)
-
-unfold
-let quad32_map2 (f:nat32 -> nat32 -> nat32) (x y:quad32) : quad32 =
-  let Quad32 x0 x1 x2 x3 = x in
-  let Quad32 y0 y1 y2 y3 = y in
-  Quad32 (f x0 y0) (f x1 y1) (f x2 y2) (f x3 y3)
-
-let quad32_xor (x y:quad32) : quad32 = quad32_map2 nat32_xor x y
-
-let select_word (q:quad32) (selector:twobits) =
-  match selector with
-  | 0 -> q.lo
-  | 1 -> q.mid_lo
-  | 2 -> q.mid_hi
-  | 3 -> q.hi
-
-let insert_nat32 (q:quad32) (n:nat32) (i:twobits) =
-  match i with 
-  | 0 -> Quad32 n q.mid_lo q.mid_hi q.hi
-  | 1 -> Quad32 q.lo n q.mid_hi q.hi
-  | 2 -> Quad32 q.lo q.mid_lo n q.hi
-  | 3 -> Quad32 q.lo q.mid_lo q.mid_hi n
+let select_word (q:quad32) (selector:twobits) : nat32 = four_select q selector
+let insert_nat32 (q:quad32) (n:nat32) (i:twobits) : quad32 = four_insert q n i
 
 open FStar.Seq
 
-assume val be_bytes_to_nat32 (b:seq nat8 {length b == 4}) : Tot nat32
-assume val nat32_to_be_bytes (n:nat32) : Tot (b:seq nat8 { length b = 4 /\ be_bytes_to_nat32 b == n }) 
+let be_bytes_to_nat32 (b:seq4 nat8) : Tot nat32 =
+  four_to_nat 8 (seq_to_four_BE b)
+
+let nat32_to_be_bytes (n:nat32) : Tot (b:seq4 nat8 { be_bytes_to_nat32 b == n }) =
+  let b = four_to_seq_BE (nat_to_four 8 n) in
+  assume (be_bytes_to_nat32 b == n);
+  b
 
 assume val be_bytes_to_nat32_to_be_bytes (b:seq nat8 {length b == 4}) : 
   Lemma (nat32_to_be_bytes (be_bytes_to_nat32 b) == b)
@@ -98,12 +53,8 @@ let reverse_bytes_nat32 (n:nat32) : Tot (nat32) =
   be_bytes_to_nat32 (reverse_seq (nat32_to_be_bytes n))
 
 let reverse_bytes_quad32 (q:quad32) : quad32 =
-  Quad32 (reverse_bytes_nat32 q.hi)
-	 (reverse_bytes_nat32 q.mid_hi)
-	 (reverse_bytes_nat32 q.mid_lo)
-	 (reverse_bytes_nat32 q.lo)
+  four_reverse (four_map reverse_bytes_nat32 q)
 
 // Reverses the bytes in each nat32, but not the nat32s themselves
-let rec reverse_bytes_nat32_seq (s:seq nat32) : Tot (s':seq nat32 { length s == length s' }) (decreases %[length s]) =
-  if length s = 0 then createEmpty
-  else (lemma_empty s; cons (reverse_bytes_nat32 (head s)) (reverse_bytes_nat32_seq (tail s)))
+let reverse_bytes_nat32_seq (s:seq nat32) : s':seq nat32 { length s == length s' } =
+  seq_map reverse_bytes_nat32 s
