src/arch/x64/X64.Leakage_Ins_i.fst
@@ -191,8 +191,8 @@ let lemma_add_same_public ts fuel ins s1 s2 =
 	  let v12 = eval_operand src2 s1.state in
 	  let v21 = eval_operand src1 s2.state in
 	  let v22 = eval_operand src2 s2.state in	  
-	  let v1 = (v11 + v12) % nat64_max in
-	  let v2 = (v21 + v22) % nat64_max in
+	  let v1 = (v11 + v12) % pow2_64 in
+	  let v2 = (v21 + v22) % pow2_64 in
  	  lemma_store_load_mem64 ptr1 v1 s1.state.mem;
 	  lemma_store_load_mem64 ptr2 v2 s2.state.mem;
 	  lemma_valid_store_mem64 ptr1 v1 s1.state.mem;
@@ -222,8 +222,8 @@ let lemma_sub_same_public ts fuel ins s1 s2 =
 	  let v12 = eval_operand src2 s1.state in
 	  let v21 = eval_operand src1 s2.state in
 	  let v22 = eval_operand src2 s2.state in	  
-	  let v1 = (v11 - v12) % nat64_max in
-	  let v2 = (v21 - v22) % nat64_max in
+	  let v1 = (v11 - v12) % pow2_64 in
+	  let v2 = (v21 - v22) % pow2_64 in
  	  lemma_store_load_mem64 ptr1 v1 s1.state.mem;
 	  lemma_store_load_mem64 ptr2 v2 s2.state.mem;
 	  lemma_valid_store_mem64 ptr1 v1 s1.state.mem;
@@ -315,8 +315,8 @@ let lemma_addlea_same_public ts fuel ins s1 s2 =
 	  let v12 = eval_operand src2 s1.state in
 	  let v21 = eval_operand src1 s2.state in
 	  let v22 = eval_operand src2 s2.state in	  
-	  let v1 = (v11 + v12) % nat64_max in
-	  let v2 = (v21 + v22) % nat64_max in
+	  let v1 = (v11 + v12) % pow2_64 in
+	  let v2 = (v21 + v22) % pow2_64 in
  	  lemma_store_load_mem64 ptr1 v1 s1.state.mem;
 	  lemma_store_load_mem64 ptr2 v2 s2.state.mem;
 	  lemma_valid_store_mem64 ptr1 v1 s1.state.mem;
@@ -348,8 +348,8 @@ let lemma_addcarry_same_public ts fuel ins s1 s2 =
 	  let v12 = eval_operand src2 s1.state in
 	  let v21 = eval_operand src1 s2.state in
 	  let v22 = eval_operand src2 s2.state in	  
-	  let v1 = (v11 + v12 + c1) % nat64_max in
-	  let v2 = (v21 + v22 + c2) % nat64_max in
+	  let v1 = (v11 + v12 + c1) % pow2_64 in
+	  let v2 = (v21 + v22 + c2) % pow2_64 in
  	  lemma_store_load_mem64 ptr1 v1 s1.state.mem;
 	  lemma_store_load_mem64 ptr2 v2 s2.state.mem;
 	  lemma_valid_store_mem64 ptr1 v1 s1.state.mem;
