src/crypto/aes/GCM_s.fst
@@ -3,6 +3,7 @@ module GCM_s
 // IMPORTANT: Following NIST's specification, this spec is written assuming a big-endian mapping from bytes to quad32s
 //            Since the AES spec (AES_s) is in little-endian, we need to byteswap each time we call AES
 
+open Words_s
 open Types_s
 open AES_s
 open GCTR_s
@@ -13,10 +14,10 @@ unfold type gcm_plain = gctr_plain
 unfold type gcm_auth = gctr_plain
 
 let gcm_encrypt (alg:algorithm) (key:aes_key alg) (iv:quad32) (p:gcm_plain) (a:gcm_auth)  =
-  let h = aes_encrypt alg (reverse_bytes_nat32_seq key) (Quad32 0 0 0 0) in
-  let j0 = Quad32 1 iv.mid_lo iv.mid_hi iv.hi in
+  let h = aes_encrypt alg (reverse_bytes_nat32_seq key) (Mkfour 0 0 0 0) in
+  let j0 = Mkfour 1 iv.lo1 iv.hi2 iv.hi3 in
   let c = gctr_encrypt (inc32 j0 1) p alg key in
-  let hash_input = append a (append c (create 1 (Quad32 0 (length c % nat32_max) 0 (length a)))) in // Mod is needed, since F* can't see length c fits without a lemma
+  let hash_input = append a (append c (create 1 (Mkfour 0 (length c % pow2_32) 0 (length a)))) in // Mod is needed, since F* can't see length c fits without a lemma
   let s = ghash h hash_input in
   let t = gctr_encrypt j0 (create 1 s) alg key in
   c, t
