src/crypto/aes/GHash_i.fst
@@ -1,5 +1,6 @@
 module GHash_i
 
+open Words_s
 open Types_s
 open GHash_s
 open GF128_s
@@ -20,7 +21,7 @@ let rec ghash_incremental (h:quad32) (y_prev:quad32) (x:ghash_plain) : Tot quad3
   gf128_to_quad32 (gf128_mul xor_poly h_poly)
 
 let rec ghash_incremental_to_ghash (h:quad32) (x:ghash_plain) :
-  Lemma(ensures ghash_incremental h (Quad32 0 0 0 0) x == ghash h x)
+  Lemma(ensures ghash_incremental h (Mkfour 0 0 0 0) x == ghash h x)
        (decreases %[length x])
   =
   if length x = 1 then ()
@@ -49,7 +50,7 @@ let ghash_incremental0 (h:quad32) (y_prev:quad32) (x:seq quad32) : quad32 =
   if length x > 0 then ghash_incremental h y_prev x else y_prev
 
 let lemma_hash_append3 (h y_init y_mid1 y_mid2 y_final:quad32) (s1 s2 s3:seq quad32) : Lemma
-  (requires y_init = Quad32 0 0 0 0 /\
+  (requires y_init = Mkfour 0 0 0 0 /\
             y_mid1 = ghash_incremental0 h y_init s1 /\
             y_mid2 = ghash_incremental0 h y_mid1 s2 /\
             length s3 > 0 /\
@@ -59,15 +60,15 @@ let lemma_hash_append3 (h y_init y_mid1 y_mid2 y_final:quad32) (s1 s2 s3:seq qua
   let s23 = append s2 s3 in
   let s123 = append s1 s23 in
   if length s1 = 0 then (
-    assert(eq s123 s23);
+    assert(equal s123 s23);
     if length s2 = 0 then (
-      assert(eq s123 s3);
+      assert(equal s123 s3);
       ghash_incremental_to_ghash h s3
     ) else
       lemma_hash_append h y_mid1 s2 s3;
       ghash_incremental_to_ghash h s23
   ) else if length s2 = 0 then (
-    assert(eq s123 (append s1 s3));
+    assert(equal s123 (append s1 s3));
     lemma_hash_append h y_init s1 s3;
     ghash_incremental_to_ghash h (append s1 s3)
   ) else (
