src/crypto/aes/GHash_s.fst
@@ -1,5 +1,6 @@
 module GHash_s
 
+open Words_s
 open Types_s
 open GF128_s
 open Collections.Seqs_s
@@ -12,7 +13,7 @@ let rec ghash (h:quad32) (x:ghash_plain) : Tot quad32 (decreases %[length x]) =
   let h_poly = gf128_of_quad32 h in
   let y_i_minus_1 =
     (if length x = 1 then
-       Quad32 0 0 0 0
+       Mkfour 0 0 0 0
      else
        ghash h (all_but_last x)) in
   let x_i = last x in
