src/crypto/aes/aes-x64/FastMul_helpers_i.fst
@@ -1,5 +1,6 @@
 module FastMul_helpers_i
 
+open Words_s
 open Types_s
 open FStar.Mul
 open FStar.Tactics
@@ -8,18 +9,18 @@ open CanonCommSemiring
 let int_canon = fun _ -> canon_semiring int_cr
 
 let simple_helper (a0 b0 b1 a0b0_lo a0b0_hi a0b1_lo a0b1_hi sum:nat64) (overflow:bool) : Lemma
-  (requires nat64_max * a0b0_hi + a0b0_lo == a0 * b0 /\
-            nat64_max * a0b1_hi + a0b1_lo == a0 * b1 /\
+  (requires pow2_64 * a0b0_hi + a0b0_lo == a0 * b0 /\
+            pow2_64 * a0b1_hi + a0b1_lo == a0 * b1 /\
             sum == add_wrap (add_wrap a0b1_lo a0b0_hi) 0 /\
-            overflow == (a0b1_lo + a0b0_hi >= nat64_max))
-  (ensures (let b = b0 + nat64_max * b1 in
+            overflow == (a0b1_lo + a0b0_hi >= pow2_64))
+  (ensures (let b = b0 + pow2_64 * b1 in
             let overflow_v = if overflow then 1 else 0 in
-            a0 * b == a0b0_lo + nat64_max * sum + nat128_max * (a0b1_hi + overflow_v)))
+            a0 * b == a0b0_lo + pow2_64 * sum + pow2_128 * (a0b1_hi + overflow_v)))
   =
-  let b = b0 + nat64_max * b1 in
+  let b = b0 + pow2_64 * b1 in
   let overflow_v = if overflow then 1 else 0 in
   let lhs = a0 * b in
-  let rhs = a0b0_lo + nat64_max * sum + nat128_max * (a0b1_hi + overflow_v) in
+  let rhs = a0b0_lo + pow2_64 * sum + pow2_128 * (a0b1_hi + overflow_v) in
   assert_by_tactic (lhs == rhs)
     int_canon;
   ()
