src/crypto/poly1305/Poly1305.Spec_s.fst
@@ -1,10 +1,11 @@
 module Poly1305.Spec_s
 
 open FStar.Mul
+open Words_s
 open Types_s
 
 let modp'(x:int):int =
-  x % (nat128_max * 4 - 5)
+  x % (pow2_128 * 4 - 5)
 
 let and128 (x:nat128) (y:nat128) : nat128 =
   iand x y
@@ -20,12 +21,12 @@ let poly1305_hash (key_r:nat128) (key_s:nat128) (inp:int->nat128) (len:nat) :int
   let r = iand key_r 0x0ffffffc0ffffffc0ffffffc0fffffff in
   let nBlocks = len / 16 in
   let nExtra = len % 16 in
-  let padBlocks = nat128_max in
+  let padBlocks = pow2_128 in
   let hBlocks = poly1305_hash_blocks 0 padBlocks r inp nBlocks in
   if nExtra = 0 then
-    (hBlocks + key_s) % nat128_max
+    (hBlocks + key_s) % pow2_128
   else
     let k = nBlocks in
     let padLast = pow2(nExtra * 8) in
     let hLast = modp' ((hBlocks + padLast + ((inp k) % padLast)) * r) in
-    (hLast + key_s) % nat128_max
+    (hLast + key_s) % pow2_128
